Remove the schedule oracle

src/hls/RTLPargen.v
@@ -16,19 +16,531 @@
  * along with this program.  If not, see <https://www.gnu.org/licenses/>.
  *)
 
+Require compcert.backend.Registers.
 Require Import compcert.common.AST.
+Require Import compcert.common.Globalenvs.
+Require compcert.common.Memory.
+Require Import compcert.common.Values.
+Require Import compcert.lib.Floats.
+Require Import compcert.lib.Integers.
 Require Import compcert.lib.Maps.
+Require compcert.verilog.Op.
 
 Require Import vericert.common.Vericertlib.
 Require Import vericert.hls.RTLBlock.
+Require Import vericert.hls.RTLBlockInstr.
 Require Import vericert.hls.RTLPar.
-Require Import vericert.hls.Scheduleoracle.
+
+(*|
+Schedule Oracle
+===============
+
+This oracle determines if a schedule was valid by performing symbolic execution on the input and
+output and showing that these behave the same.  This acts on each basic block separately, as the
+rest of the functions should be equivalent.
+|*)
+
+Definition reg := positive.
+
+Inductive resource : Set :=
+| Reg : reg -> resource
+| Mem : resource.
+
+(*|
+The following defines quite a few equality comparisons automatically, however, these can be
+optimised heavily if written manually, as their proofs are not needed.
+|*)
+
+Lemma resource_eq : forall (r1 r2 : resource), {r1 = r2} + {r1 <> r2}.
+Proof.
+  decide equality. apply Pos.eq_dec.
+Defined.
+
+Lemma comparison_eq: forall (x y : comparison), {x = y} + {x <> y}.
+Proof.
+  decide equality.
+Defined.
+
+Lemma condition_eq: forall (x y : Op.condition), {x = y} + {x <> y}.
+Proof.
+  generalize comparison_eq; intro.
+  generalize Int.eq_dec; intro.
+  generalize Int64.eq_dec; intro.
+  decide equality.
+Defined.
+
+Lemma addressing_eq : forall (x y : Op.addressing), {x = y} + {x <> y}.
+Proof.
+  generalize Int.eq_dec; intro.
+  generalize AST.ident_eq; intro.
+  generalize Z.eq_dec; intro.
+  generalize Ptrofs.eq_dec; intro.
+  decide equality.
+Defined.
+
+Lemma typ_eq : forall (x y : AST.typ), {x = y} + {x <> y}.
+Proof.
+  decide equality.
+Defined.
+
+Lemma operation_eq: forall (x y : Op.operation), {x = y} + {x <> y}.
+Proof.
+  generalize Int.eq_dec; intro.
+  generalize Int64.eq_dec; intro.
+  generalize Float.eq_dec; intro.
+  generalize Float32.eq_dec; intro.
+  generalize AST.ident_eq; intro.
+  generalize condition_eq; intro.
+  generalize addressing_eq; intro.
+  generalize typ_eq; intro.
+  decide equality.
+Defined.
+
+Lemma memory_chunk_eq : forall (x y : AST.memory_chunk), {x = y} + {x <> y}.
+Proof.
+  decide equality.
+Defined.
+
+Lemma list_typ_eq: forall (x y : list AST.typ), {x = y} + {x <> y}.
+Proof.
+  generalize typ_eq; intro.
+  decide equality.
+Defined.
+
+Lemma option_typ_eq : forall (x y : option AST.typ), {x = y} + {x <> y}.
+Proof.
+  generalize typ_eq; intro.
+  decide equality.
+Defined.
+
+Lemma signature_eq: forall (x y : AST.signature), {x = y} + {x <> y}.
+Proof.
+  repeat decide equality.
+Defined.
+
+Lemma list_operation_eq : forall (x y : list Op.operation), {x = y} + {x <> y}.
+Proof.
+  generalize operation_eq; intro.
+  decide equality.
+Defined.
+
+Lemma list_reg_eq : forall (x y : list reg), {x = y} + {x <> y}.
+Proof.
+  generalize Pos.eq_dec; intros.
+  decide equality.
+Defined.
+
+Lemma sig_eq : forall (x y : AST.signature), {x = y} + {x <> y}.
+Proof.
+  repeat decide equality.
+Defined.
+
+Lemma instr_eq: forall (x y : instr), {x = y} + {x <> y}.
+Proof.
+  generalize Pos.eq_dec; intro.
+  generalize typ_eq; intro.
+  generalize Int.eq_dec; intro.
+  generalize memory_chunk_eq; intro.
+  generalize addressing_eq; intro.
+  generalize operation_eq; intro.
+  generalize condition_eq; intro.
+  generalize signature_eq; intro.
+  generalize list_operation_eq; intro.
+  generalize list_reg_eq; intro.
+  generalize AST.ident_eq; intro.
+  decide equality.
+Defined.
+
+Lemma cf_instr_eq: forall (x y : cf_instr), {x = y} + {x <> y}.
+Proof.
+  generalize Pos.eq_dec; intro.
+  generalize typ_eq; intro.
+  generalize Int.eq_dec; intro.
+  generalize Int64.eq_dec; intro.
+  generalize Float.eq_dec; intro.
+  generalize Float32.eq_dec; intro.
+  generalize Ptrofs.eq_dec; intro.
+  generalize memory_chunk_eq; intro.
+  generalize addressing_eq; intro.
+  generalize operation_eq; intro.
+  generalize condition_eq; intro.
+  generalize signature_eq; intro.
+  generalize list_operation_eq; intro.
+  generalize list_reg_eq; intro.
+  generalize AST.ident_eq; intro.
+  repeat decide equality.
+Defined.
+
+(*|
+We then create equality lemmas for a resource and a module to index resources uniquely.  The
+indexing is done by setting Mem to 1, whereas all other infinitely many registers will all be
+shifted right by 1.  This means that they will never overlap.
+|*)
+
+Module R_indexed.
+  Definition t := resource.
+  Definition index (rs: resource) : positive :=
+    match rs with
+    | Reg r => xO r
+    | Mem => 1%positive
+    end.
+
+  Lemma index_inj:  forall (x y: t), index x = index y -> x = y.
+  Proof. destruct x; destruct y; crush. Qed.
+
+  Definition eq := resource_eq.
+End R_indexed.
+
+(*|
+We can then create expressions that mimic the expressions defined in RTLBlock and RTLPar, which use
+expressions instead of registers as their inputs and outputs.  This means that we can accumulate all
+the results of the operations as general expressions that will be present in those registers.
+
+- Ebase: the starting value of the register.
+- Eop: Some arithmetic operation on a number of registers.
+- Eload: A load from a memory location into a register.
+- Estore: A store from a register to a memory location.
+
+Then, to make recursion over expressions easier, expression_list is also defined in the datatype, as
+that enables mutual recursive definitions over the datatypes.
+|*)
+
+Inductive expression : Set :=
+| Ebase : resource -> expression
+| Eop : Op.operation -> expression_list -> expression
+| Eload : AST.memory_chunk -> Op.addressing -> expression_list -> expression -> expression
+| Estore : expression -> AST.memory_chunk -> Op.addressing -> expression_list -> expression -> expression
+with expression_list : Set :=
+| Enil : expression_list
+| Econs : expression -> expression_list -> expression_list.
+
+(*|
+Using IMap we can create a map from resources to any other type, as resources can be uniquely
+identified as positive numbers.
+|*)
+
+Module Rtree := ITree(R_indexed).
+
+Definition forest : Type := Rtree.t expression.
+
+Definition regset := Registers.Regmap.t val.
+
+Definition get_forest v f :=
+  match Rtree.get v f with
+  | None => Ebase v
+  | Some v' => v'
+  end.
+
+Notation "a # b" := (get_forest b a) (at level 1).
+Notation "a # b <- c" := (Rtree.set b c a) (at level 1, b at next level).
+
+Record sem_state := mk_sem_state {
+                    sem_state_stackp : val;
+                    sem_state_regset : regset;
+                    sem_state_memory : Memory.mem
+                    }.
+
+(*|
+Finally we want to define the semantics of execution for the expressions with symbolic values, so
+the result of executing the expressions will be an expressions.
+|*)
+
+Section SEMANTICS.
+
+Context (A : Set) (genv : Genv.t A unit).
+
+Inductive sem_value :
+      val -> sem_state -> expression -> val -> Prop :=
+  | Sbase_reg:
+          forall parent st r,
+          sem_value parent st (Ebase (Reg r)) (Registers.Regmap.get r (sem_state_regset st))
+  | Sop:
+          forall parent st op args v lv,
+          sem_val_list parent st args lv ->
+          Op.eval_operation genv (sem_state_stackp st) op lv (sem_state_memory st) = Some v ->
+          sem_value parent st (Eop op args) v
+  | Sload :
+          forall parent st mem_exp addr chunk args a v m' lv ,
+          sem_mem parent st mem_exp m' ->
+          sem_val_list parent st args lv ->
+          Op.eval_addressing genv (sem_state_stackp st) addr lv = Some a ->
+          Memory.Mem.loadv chunk m' a = Some v ->
+          sem_value parent st (Eload chunk addr args mem_exp) v
+with sem_mem :
+           val -> sem_state -> expression -> Memory.mem -> Prop :=
+  | Sstore :
+          forall parent st mem_exp val_exp m'' addr v a m' chunk args lv,
+          sem_mem parent st mem_exp m' ->
+          sem_value parent st val_exp v ->
+          sem_val_list parent st args lv ->
+          Op.eval_addressing genv (sem_state_stackp st) addr lv = Some a ->
+          Memory.Mem.storev chunk m' a v = Some m'' ->
+          sem_mem parent st (Estore mem_exp chunk addr args val_exp) m''
+    | Sbase_mem :
+            forall parent st m,
+            sem_mem parent st (Ebase Mem) m
+with sem_val_list :
+           val -> sem_state -> expression_list -> list val -> Prop :=
+    | Snil :
+            forall parent st,
+            sem_val_list parent st Enil nil
+    | Scons :
+            forall parent st e v l lv,
+            sem_value parent st e v ->
+            sem_val_list parent st l lv ->
+            sem_val_list parent st (Econs e l) (v :: lv).
+
+Inductive sem_regset :
+   val -> sem_state -> forest -> regset -> Prop :=
+  | Sregset:
+        forall parent st f rs',
+        (forall x, sem_value parent st (f # (Reg x)) (Registers.Regmap.get x rs')) ->
+        sem_regset parent st f rs'.
+
+Inductive sem :
+   val -> sem_state -> forest -> sem_state -> Prop :=
+  | Sem:
+        forall st rs' fr' m' f parent,
+        sem_regset parent st f rs' ->
+        sem_mem parent st (f # Mem) m' ->
+        sem parent st fr' (mk_sem_state (sem_state_stackp st) rs' m').
+
+
+End SEMANTICS.
+
+Fixpoint beq_expression (e1 e2: expression) {struct e1}: bool :=
+  match e1, e2 with
+  | Ebase r1, Ebase r2 => if resource_eq r1 r2 then true else false
+  | Eop op1 el1, Eop op2 el2 =>
+      if operation_eq op1 op2 then beq_expression_list el1 el2 else false
+  | Eload chk1 addr1 el1 e1, Eload chk2 addr2 el2 e2 =>
+      if memory_chunk_eq chk1 chk2
+      then if addressing_eq addr1 addr2
+      then if beq_expression_list el1 el2
+      then beq_expression e1 e2 else false else false else false
+  | Estore m1 chk1 addr1 el1 e1, Estore m2 chk2 addr2 el2 e2=>
+      if memory_chunk_eq chk1 chk2
+      then if addressing_eq addr1 addr2
+      then if beq_expression_list el1 el2
+      then if beq_expression m1 m2
+      then beq_expression e1 e2 else false else false else false else false
+  | _, _ => false
+  end
+with beq_expression_list (el1 el2: expression_list) {struct el1} : bool :=
+  match el1, el2 with
+  | Enil, Enil => true
+  | Econs e1 t1, Econs e2 t2 => beq_expression e1 e2 && beq_expression_list t1 t2
+  | _, _ => false
+  end.
+
+Scheme expression_ind2 := Induction for expression Sort Prop
+  with expression_list_ind2 := Induction for expression_list Sort Prop.
+
+Lemma beq_expression_correct:
+  forall e1 e2, beq_expression e1 e2 = true -> e1 = e2.
+Proof.
+  intro e1;
+  apply expression_ind2 with
+      (P := fun (e1 : expression) =>
+            forall e2, beq_expression e1 e2 = true -> e1 = e2)
+      (P0 := fun (e1 : expression_list) =>
+             forall e2, beq_expression_list e1 e2 = true -> e1 = e2); simplify;
+    repeat match goal with
+           | [ H : context[match ?x with _ => _ end] |- _ ] => destruct x eqn:?
+           | [ H : context[if ?x then _ else _] |- _ ] => destruct x eqn:?
+           end; subst; f_equal; crush.
+Qed.
+
+Definition empty : forest := Rtree.empty _.
+
+(*|
+This function checks if all the elements in [fa] are in [fb], but not the other way round.
+|*)
+
+Definition check := Rtree.beq beq_expression.
+
+Lemma check_correct: forall (fa fb : forest) (x : resource),
+  check fa fb = true -> (forall x, fa # x = fb # x).
+Proof.
+  unfold check, get_forest; intros;
+  pose proof beq_expression_correct;
+  match goal with
+    [ Hbeq : context[Rtree.beq], y : Rtree.elt |- _ ] =>
+    apply (Rtree.beq_sound beq_expression fa fb) with (x := y) in Hbeq
+  end;
+  repeat destruct_match; crush.
+Qed.
+
+Lemma get_empty:
+  forall r, empty#r = Ebase r.
+Proof.
+  intros; unfold get_forest;
+  destruct_match; auto; [ ];
+  match goal with
+    [ H : context[Rtree.get _ empty] |- _ ] => rewrite Rtree.gempty in H
+  end; discriminate.
+Qed.
+
+Fixpoint beq2 {A B : Type} (beqA : A -> B -> bool) (m1 : PTree.t A) (m2 : PTree.t B) {struct m1} : bool :=
+  match m1, m2 with
+  | PTree.Leaf, _ => PTree.bempty m2
+  | _, PTree.Leaf => PTree.bempty m1
+  | PTree.Node l1 o1 r1, PTree.Node l2 o2 r2 =>
+    match o1, o2 with
+    | None, None => true
+    | Some y1, Some y2 => beqA y1 y2
+    | _, _ => false
+    end
+    && beq2 beqA l1 l2 && beq2 beqA r1 r2
+  end.
+
+Lemma beq2_correct:
+  forall A B beqA m1 m2,
+    @beq2 A B beqA m1 m2 = true <->
+    (forall (x: PTree.elt),
+        match PTree.get x m1, PTree.get x m2 with
+        | None, None => True
+        | Some y1, Some y2 => beqA y1 y2 = true
+        | _, _ => False
+        end).
+Proof.
+  induction m1; intros.
+  - simpl. rewrite PTree.bempty_correct. split; intros.
+    rewrite PTree.gleaf. rewrite H. auto.
+    generalize (H x). rewrite PTree.gleaf. destruct (PTree.get x m2); tauto.
+  - destruct m2.
+    + unfold beq2. rewrite PTree.bempty_correct. split; intros.
+      rewrite H. rewrite PTree.gleaf. auto.
+      generalize (H x). rewrite PTree.gleaf. destruct (PTree.get x (PTree.Node m1_1 o m1_2)); tauto.
+    + simpl. split; intros.
+      * destruct (andb_prop _ _ H). destruct (andb_prop _ _ H0).
+        rewrite IHm1_1 in H3. rewrite IHm1_2 in H1.
+        destruct x; simpl. apply H1. apply H3.
+        destruct o; destruct o0; auto || congruence.
+      * apply andb_true_intro. split. apply andb_true_intro. split.
+        generalize (H xH); simpl. destruct o; destruct o0; tauto.
+        apply IHm1_1. intros; apply (H (xO x)).
+        apply IHm1_2. intros; apply (H (xI x)).
+Qed.
+
+Lemma map0:
+  forall r,
+  empty # r = Ebase r.
+Proof. intros; eapply get_empty. Qed.
+
+Lemma map1:
+  forall w dst dst',
+  dst <> dst' ->
+  (empty # dst <- w) # dst' = Ebase dst'.
+Proof. intros; unfold get_forest; rewrite Rtree.gso; auto; apply map0. Qed.
+
+Lemma genmap1:
+  forall (f : forest) w dst dst',
+  dst <> dst' ->
+  (f # dst <- w) # dst' = f # dst'.
+Proof. intros; unfold get_forest; rewrite Rtree.gso; auto. Qed.
+
+Lemma map2:
+  forall (v : expression) x rs,
+  (rs # x <- v) # x = v.
+Proof. intros; unfold get_forest; rewrite Rtree.gss; trivial. Qed.
+
+Lemma tri1:
+  forall x y,
+  Reg x <> Reg y -> x <> y.
+Proof. unfold not; intros; subst; auto. Qed.
+
+(*|
+Update functions.
+|*)
+
+Fixpoint list_translation (l : list reg) (f : forest) {struct l} : expression_list :=
+  match l with
+  | nil => Enil
+  | i :: l => Econs (f # (Reg i)) (list_translation l f)
+  end.
+
+Definition update (f : forest) (i : instr) : forest :=
+  match i with
+  | RBnop => f
+  | RBop op rl r =>
+    f # (Reg r) <- (Eop op (list_translation rl f))
+  | RBload chunk addr rl r =>
+    f # (Reg r) <- (Eload chunk addr (list_translation rl f) (f # Mem))
+  | RBstore chunk addr rl r =>
+    f # Mem <- (Estore (f # Mem) chunk addr (list_translation rl f) (f # (Reg r)))
+  end.
+
+(*|
+Implementing which are necessary to show the correctness of the translation validation by showing
+that there aren't any more effects in the resultant RTLPar code than in the RTLBlock code.
+|*)
+
+
+
+(*|
+Get a sequence from the basic block.
+|*)
+
+Fixpoint abstract_sequence (f : forest) (b : list instr) : forest :=
+  match b with
+  | nil => f
+  | i :: l => abstract_sequence (update f i) l
+  end.
+
+Fixpoint abstract_sequence_par (f : forest) (b : list (list instr)) : forest :=
+  match b with
+  | nil => f
+  | i :: l => abstract_sequence_par (abstract_sequence f i) l
+  end.
+
+(*|
+Check equivalence of control flow instructions.  As none of the basic blocks should have been moved,
+none of the labels should be different, meaning the control-flow instructions should match exactly.
+|*)
+
+Definition check_control_flow_instr (c1 c2: cf_instr) : bool :=
+  if cf_instr_eq c1 c2 then true else false.
+
+(*|
+We define the top-level oracle that will check if two basic blocks are equivalent after a scheduling
+transformation.
+|*)
+
+Definition schedule_oracle (bb: RTLBlock.bblock) (bbt: RTLPar.bblock) : bool :=
+  check (abstract_sequence empty (bb_body bb))
+        (abstract_sequence_par empty (bb_body bbt)).
+
+Definition check_scheduled_trees := beq2 schedule_oracle.
+
+Ltac solve_scheduled_trees_correct :=
+  intros; unfold check_scheduled_trees in *;
+  match goal with
+  | [ H: context[beq2 _ _ _], x: positive |- _ ] =>
+    rewrite beq2_correct in H; specialize (H x)
+  end; repeat destruct_match; crush.
+
+Lemma check_scheduled_trees_correct:
+  forall f1 f2,
+    check_scheduled_trees f1 f2 = true ->
+    (forall x y1,
+        PTree.get x f1 = Some y1 ->
+        exists y2, PTree.get x f2 = Some y2 /\ schedule_oracle y1 y2 = true).
+Proof. solve_scheduled_trees_correct; eexists; crush. Qed.
+
+Lemma check_scheduled_trees_correct2:
+  forall f1 f2,
+    check_scheduled_trees f1 f2 = true ->
+    (forall x,
+        PTree.get x f1 = None ->
+        PTree.get x f2 = None).
+Proof. solve_scheduled_trees_correct. Qed.
 
 Parameter schedule : RTLBlock.function -> RTLPar.function.
 
-Definition transl_function (f : RTLBlock.function) : Errors.res RTLPar.function :=
+Definition transl_function (f: RTLBlock.function) : Errors.res RTLPar.function :=
   let tf := schedule f in
-  if beq2 schedule_oracle f.(RTLBlock.fn_code) tf.(fn_code) then
+  if check_scheduled_trees f.(RTLBlock.fn_code) tf.(fn_code) then
     Errors.OK tf
   else
     Errors.Error (Errors.msg "RTLPargen: Could not prove the blocks equivalent.").
